evaluateLagrangePolyOutOfDomain mid => low (#37)

src/specs/EvaluateLagrangePolyOutOfDomain.ec
@@ -1,6 +1,10 @@
 pragma Goals:printall.
 
-require        Constants.
+require import AllCore.
+require import Int.
+require import IntDiv.
+require import Constants.
+require import Utils.
 require import Modexp.
 require import PurePrimops.
 require import RevertWithMessage.
@@ -8,6 +12,8 @@ require import UInt256.
 require import Verifier.
 require import VerifierConsts.
 require import YulPrimops.
+
+import MemoryMap.
 
 module EvaluateLagrangePolyOutOfDomain = {
   proc low(polyNum: uint256, at: uint256): uint256 = {
@@ -33,6 +39,50 @@ module EvaluateLagrangePolyOutOfDomain = {
     ret <- (PurePrimops.mulmod ret denominator R_MOD);
     return ret;
   }
+  
+  proc mid'(polyNum: int, at: int): int option = {
+    var r, omegaPolyNum, atDomainSize, zd1, num, den, inv;
+
+    omegaPolyNum <@ Modexp.mid(OMEGA,polyNum);
+    atDomainSize <@ Modexp.mid(at, DOMAIN_SIZE); 
+
+    zd1 <- (atDomainSize - 1) %% R;
+    if(zd1 = 0) { (* (at ^ DOMAIN_SIZE) - 1 = 0 *)
+      r <- None;
+    } else {
+      num <- (omegaPolyNum * zd1) %% R;
+      den <- (DOMAIN_SIZE * (at - omegaPolyNum)) %% R;
+      inv <@ Modexp.mid(den, R - 2);
+      r <- Some ((num * inv) %% R);
+      (* ((OMEGA ^ polyNum) * (atDomainSize - 1))
+        ----------------------------------------
+        (DOMAIN_SIZE * (at - (OMEGA ^ polyNum)))
+      *)
+    }  
+    return r;
+  }
+
+  proc mid(polyNum: int, at: int): int option = {
+    var r, omegaPolyNum, atDomainSize, zd1, num, den, inv;
+
+    omegaPolyNum <- (OMEGA^polyNum) %% R;
+    atDomainSize <- (at^DOMAIN_SIZE) %% R; 
+
+    zd1 <- (atDomainSize - 1) %% R;
+    if(zd1 = 0) { (* (at ^ DOMAIN_SIZE) - 1 = 0 *)
+      r <- None;
+    } else {
+      num <- (omegaPolyNum * zd1) %% R;
+      den <- (DOMAIN_SIZE * (at - omegaPolyNum)) %% R;
+      inv <- (den^(R - 2)) %% R;
+      r <- Some ((num * inv) %% R);
+      (* ((OMEGA ^ polyNum) * (atDomainSize - 1))
+        ----------------------------------------
+        (DOMAIN_SIZE * (at - (OMEGA ^ polyNum)))
+      *)
+    }  
+    return r;
+  }  
 }.
 
 lemma evaluateLagrangePolyOutOfDomain_extracted_equiv_low:
@@ -70,8 +120,172 @@ lemma evaluateLagrangePolyOutOfDomain_extracted_equiv_low:
         call revertWithMessage_extracted_equiv_low. skip. by progress.
         sp. skip. by progress.
     qed.
-        
 
-        
-        
-        
+pred lagrange_memory_footprint (initial final : mem)  =
+   exists (v1 v2 v3: uint256), final = modexp_memory_footprint initial v1 v2 v3.
+
+lemma evaluateLagrangePolyOutOfDomain_low_equiv_mid' (memory : mem) (poly256 at256: uint256):
+equiv [
+    EvaluateLagrangePolyOutOfDomain.low ~ EvaluateLagrangePolyOutOfDomain.mid' :
+      arg{1} = (poly256, at256) /\
+      arg{2} = (to_uint poly256, to_uint at256)%W256 /\
+      !Primops.reverted{1} /\
+      Primops.memory{1} = memory
+      ==>
+      ((!Primops.reverted{1} /\
+        lagrange_memory_footprint memory Primops.memory{1} /\
+        res{2} = Some (to_uint res{1})%W256 /\ 0 <= to_uint res{1} < R)
+      \/
+      (Primops.reverted{1} /\ res{2} = None))
+    ].
+proof. proc.
+    
+seq 2 1 : (
+  (polyNum{1}, at{1}) = (poly256, at256) /\
+  (polyNum{2}, at{2}) = (to_uint poly256, to_uint at256) /\
+  !Primops.reverted{1} /\
+  ((poly256 <> W256.zero /\ Primops.memory{1} = (modexp_memory_footprint memory (W256.of_int OMEGA) polyNum{1} omegaPower{1})) 
+    \/
+  (poly256 = W256.zero /\ Primops.memory{1} = memory))
+  /\
+  omegaPower{1} = W256.of_int omegaPolyNum{2} /\ 0 <= omegaPolyNum{2} < R
+). sp.
+case (bool_of_uint256 polyNum{1}).
+(* polyNum != 0 *)
+rcondt{1} 1. by progress.
+call (modexp_low_equiv_mid memory (W256.of_int OMEGA) poly256).
+(* call{1} (modexp_pspec memory (W256.of_int OMEGA) poly256). *)
+skip. progress. by smt. left. by auto.
+rcondf{1} 1. by progress.
+inline Modexp.mid. wp. skip. progress. right. by auto.
+have ->: polyNum{1} = W256.zero. by auto. by smt().
+have ->: polyNum{1} = W256.zero. by auto. by smt().
+have ->: polyNum{1} = W256.zero. by auto. by smt().
+
+seq 1 1: (
+  (polyNum{1}, at{1}) = (poly256, at256) /\
+  (polyNum{2}, at{2}) = (to_uint poly256, to_uint at256) /\
+  !Primops.reverted{1} /\
+  Primops.memory{1} = modexp_memory_footprint memory at{1} (W256.of_int DOMAIN_SIZE) tmp267{1} /\
+  omegaPower{1} = W256.of_int omegaPolyNum{2} /\ 0 <= omegaPolyNum{2} < R /\
+  tmp267{1} = W256.of_int atDomainSize{2} /\ 0 <= atDomainSize{2} < R
+).
+wp. 
+exists* omegaPower{1}. elim* => oP.
+pose mem' := (modexp_memory_footprint memory ((of_int OMEGA))%W256 poly256 oP).
+case (poly256 = W256.zero).
+call{1} (modexp_low_equiv_mid memory at256 (W256.of_int DOMAIN_SIZE)).
+skip. progress. by smt. by smt().
+call{1} (modexp_low_equiv_mid mem' at256 (W256.of_int DOMAIN_SIZE)).
+skip. progress. by smt. by smt(). apply modexp_memory_footprint_same.
+
+seq 1 1: (#pre /\ ret{1} = W256.of_int zd1{2} /\ 0 <= zd1{2} < R).
+wp. skip. progress.
+rewrite /addmod. progress. rewrite !W256.of_uintK !R_mod_W256_R.
+have ->: (R - 1) %% W256.modulus = R - 1. by smt().
+have ->: atDomainSize{2} %% W256.modulus = atDomainSize{2}. by smt().
+by smt(). by smt(). by smt().
+
+if. progress. by smt. by smt.
+
+seq 1 1: (r{2} = None /\ Primops.reverted{1}).
+wp. call{1} revertWithMessage_low_pspec. skip. by progress.
+wp. sp. call{1} modexp_low_pspec_revert. skip. by progress.
+
+seq 1 1: (
+(polyNum{1}, at{1}) = (poly256, at256) /\
+(polyNum{2}, at{2}) = (to_uint poly256, to_uint at256) /\
+!Primops.reverted{1} /\
+Primops.memory{1} = modexp_memory_footprint memory at{1} ((of_int DOMAIN_SIZE))%W256 tmp267{1} /\
+omegaPower{1} = (of_int omegaPolyNum{2})%W256 /\ 0 <= omegaPolyNum{2} < R /\
+tmp267{1} = (of_int atDomainSize{2})%W256 /\ 0 <= atDomainSize{2} < R /\ 0 <= zd1{2} < R /\
+ret{1} = (of_int num{2})%W256 /\ 0 <= num{2} < R
+).
+wp. skip. progress.
+rewrite /mulmod. progress. rewrite !W256.of_uintK !R_mod_W256_R.
+have ->: zd1{2} %% W256.modulus = zd1{2}. by smt().
+have ->: omegaPolyNum{2} %% W256.modulus = omegaPolyNum{2}. by smt().
+by smt(). by smt(). by smt().
+
+seq 3 1: (
+#pre /\ denominator{1} = W256.of_int den{2} /\ 0 <= den{2} < R
+).
+wp. skip. progress. 
+rewrite /addmod /mulmod. progress. rewrite !W256.of_uintK !R_mod_W256_R.
+have ->: DOMAIN_SIZE %% W256.modulus = DOMAIN_SIZE. by smt().
+have ->: (R - omegaPolyNum{2}) %% W256.modulus = (R - omegaPolyNum{2}). by smt().
+rewrite !mod_R_W256_mod_R. by smt. by smt(). by smt().
+
+seq 1 1: (
+(polyNum{1}, at{1}) = (poly256, at256) /\
+(polyNum{2}, at{2}) = (to_uint poly256, to_uint at256) /\
+!Primops.reverted{1} /\
+omegaPower{1} = (of_int omegaPolyNum{2})%W256 /\
+0 <= omegaPolyNum{2} < R /\
+tmp267{1} = (of_int atDomainSize{2})%W256 /\
+0 <= atDomainSize{2} < R /\
+ret{1} = (of_int num{2})%W256 /\
+0 <= num{2} < R /\ 0 <= zd1{2} < R /\ 0 <= den{2} < R /\
+Primops.memory{1} = modexp_memory_footprint memory (of_int den{2})%W256 (W256.of_int (R - 2)) denominator{1} /\
+denominator{1} = W256.of_int inv{2} /\ 0 <= inv{2} < R
+).
+
+exists* tmp267{1}. elim* => tmp. exists* denominator{1}. elim* => d.
+pose mem' := modexp_memory_footprint memory at256 ((of_int DOMAIN_SIZE))%W256 tmp.
+call{1} (modexp_low_equiv_mid mem' d ((W256.of_int R) - (W256.of_int 2))).
+skip. progress. rewrite /mem'. by smt. by smt. apply modexp_memory_footprint_same.
+wp. skip. progress. rewrite /lagrange_memory_footprint. by smt().
+rewrite /mulmod. progress. rewrite !W256.of_uintK !R_mod_W256_R.
+have ->: num{2} %% W256.modulus = num{2}. by smt().
+have ->: inv{2} %% W256.modulus = inv{2}. by smt().
+rewrite mod_R_W256_mod_R. by reflexivity.
+rewrite /mulmod. progress. rewrite !W256.of_uintK !R_mod_W256_R.
+have ->: num{2} %% W256.modulus = num{2}. by smt().
+have ->: inv{2} %% W256.modulus = inv{2}. by smt().
+rewrite mod_R_W256_mod_R. by smt().
+rewrite /mulmod. progress. rewrite !W256.of_uintK !R_mod_W256_R.
+have ->: num{2} %% W256.modulus = num{2}. by smt().
+have ->: inv{2} %% W256.modulus = inv{2}. by smt().
+rewrite mod_R_W256_mod_R. by smt().
+qed.
+
+lemma evaluateLagrangePolyOutOfDomain_low_equiv_mid (memory : mem) (poly256 at256: uint256):
+equiv [
+    EvaluateLagrangePolyOutOfDomain.low ~ EvaluateLagrangePolyOutOfDomain.mid :
+      arg{1} = (poly256, at256) /\
+      arg{2} = (to_uint poly256, to_uint at256)%W256 /\
+      !Primops.reverted{1} /\
+      Primops.memory{1} = memory
+      ==>
+      ((!Primops.reverted{1} /\ ((to_uint at256)^DOMAIN_SIZE - 1) %% R <> 0 /\
+        lagrange_memory_footprint memory Primops.memory{1} /\
+        res{2} = Some (to_uint res{1})%W256 /\ 0 <= to_uint res{1} < R)
+      \/
+      (Primops.reverted{1} /\ ((to_uint at256)^DOMAIN_SIZE - 1) %% R = 0 /\ res{2} = None))
+    ].
+proof.
+transitivity EvaluateLagrangePolyOutOfDomain.mid'
+(
+arg{1} = (poly256, at256) /\
+      arg{2} = (to_uint poly256, to_uint at256)%W256 /\
+      !Primops.reverted{1} /\
+      Primops.memory{1} = memory
+      ==>
+      ((!Primops.reverted{1} /\
+        lagrange_memory_footprint memory Primops.memory{1} /\
+        res{2} = Some (to_uint res{1})%W256 /\ 0 <= to_uint res{1} < R)
+      \/
+      (Primops.reverted{1} /\ res{2} = None))
+)
+(
+arg{1} = (to_uint poly256, to_uint at256)%W256 /\ ={arg}
+      ==>
+      ={res} /\
+      ((((to_uint at256)^DOMAIN_SIZE - 1) %% R <> 0 /\ is_some res{2})
+      \/
+      (((to_uint at256)^DOMAIN_SIZE - 1) %% R = 0 /\ !(is_some res{2})))
+).
+progress. exists (to_uint poly256, to_uint at256). by progress.
+progress. elim H0. progress. by smt(). by smt().
+apply evaluateLagrangePolyOutOfDomain_low_equiv_mid'.
+proc. inline Modexp.mid. wp. skip. progress. by smt(). by smt(). qed.
